isSome theorems for toSingleAccept

Cslib/Computability/Machines/Turing/SingleTape/NonDeterministic.lean
@@ -8,6 +8,8 @@ module
 
 public import Cslib.Foundations.Data.Relation
 public import Cslib.Computability.Automata.NA.Basic
+public import Cslib.Computability.Automata.EpsilonNA.Basic
+public import Cslib.Computability.Automata.EpsilonNA.ToSingleAccept
 public import Cslib.Foundations.Data.BiTape
 public import Cslib.Computability.Machines.Turing.SingleTape.Defs
 
@@ -26,7 +28,7 @@ open Automata
 /-- A (single-tape) Nondeterministic Turing Machine (NTM) is a nondeterministic automaton equipped
 with a set of accepting halting states. -/
 structure SingleTapeNTM (State Symbol : Type*)
-    extends NA State (SingleTape.TrLabel State Symbol) where
+    extends NA State (TrLabel Symbol) where
   /-- The set of accepting states. -/
   accept : Set State
   /-- Proof that all accepting states are halting states. -/
@@ -34,10 +36,12 @@ structure SingleTapeNTM (State Symbol : Type*)
 
 variable {State Symbol : Type*}
 
+namespace SingleTapeNTM
+
 /-- An NTM yields a small-step operational semantics on configurations, which codifies an execution
 step. -/
 @[scoped grind =]
-def SingleTapeNTM.Red (m : SingleTapeNTM State Symbol)
+def Red (m : SingleTapeNTM State Symbol)
     (c c' : Cfg State Symbol) : Prop :=
   ∃ μ, m.Tr c.state μ c'.state ∧ -- The controller can perform the move
     μ.read = c.tape.head ∧ -- The tape has the expected symbol to be read
@@ -47,7 +51,7 @@ def SingleTapeNTM.Red (m : SingleTapeNTM State Symbol)
 execution.
 -/
 @[scoped grind =]
-def SingleTapeNTM.MRed (m : SingleTapeNTM State Symbol) :=
+def MRed (m : SingleTapeNTM State Symbol) :=
   Relation.ReflTransGen m.Red
 
 /-- An NTM is an acceptor of finite lists of symbols. -/
@@ -55,5 +59,22 @@ def SingleTapeNTM.MRed (m : SingleTapeNTM State Symbol) :=
 instance : Acceptor (SingleTapeNTM State Symbol) Symbol where
   Accepts (m : SingleTapeNTM State Symbol) (xs : List Symbol) :=
     ∃ s ∈ m.start, ∃ c', c'.state ∈ m.accept ∧ m.MRed (Cfg.mk₁ s xs) c'
+
+def _root_.Cslib.Automata.εNA.FinAcc.toNTM (a : εNA.FinAcc State Symbol) : SingleTapeNTM (Option State) Symbol :=
+  let a' := a.toSingleAccept
+  {
+    start := a'.start
+    accept := a'.accept
+    Tr
+      | s, ⟨x, none, Turing.Dir.right⟩, s' => a'.Tr s x s'
+      | _, _, _ => False
+    accept_halting := sorry
+  }
+
+open Acceptor in
+theorem pippo {a : εNA.FinAcc State Symbol} : language a.toNTM = language a := by
+  sorry
+
+end SingleTapeNTM
 
 end Cslib.Computability.Turing.SingleTape
