Cslib.lean
@@ -11,6 +11,7 @@ public import Cslib.Computability.Automata.DA.Prod
 public import Cslib.Computability.Automata.DA.ToNA
 public import Cslib.Computability.Automata.EpsilonNA.Basic
 public import Cslib.Computability.Automata.EpsilonNA.ToNA
+public import Cslib.Computability.Automata.EpsilonNA.ToSingleAccept
 public import Cslib.Computability.Automata.NA.Basic
 public import Cslib.Computability.Automata.NA.BuchiEquiv
 public import Cslib.Computability.Automata.NA.BuchiInter
